examples/tactics/StringPrinterTest.fst
@@ -3,15 +3,9 @@ module StringPrinterTest
 module U32 = FStar.UInt32
 module HST = FStar.HyperStack.ST
 module B = FStar.Buffer
-module SP = StringPrinter.RecC
-
-let test (x: U32.t) : HST.ST unit (requires (fun _ -> True)) (ensures (fun h _ h' -> B.modifies_0 h h')) =
-  SP.test x
-
-let test2 (x: U32.t) : Tot (option U32.t) =
-  SP.test_len x
+module SP = StringPrinterTest.Aux
 
 let test3 (x: U32.t) : HST.ST (option unit) (requires (fun _ -> True)) (ensures (fun h _ h' -> B.modifies_0 h h')) =
   SP.example_test x
 
-// krml -tmpdir ou -bundle 'StringPrinter.*' -drop 'FStar.Tactics.*' -drop 'FStar.Reflection.*' StringPrinterTest.fst -dast -skip-linking
+// krml -tmpdir ou -bundle 'StringPrinter.\*' -bundle StringPrinterTest.Aux -drop 'FStar.Tactics.\*' -drop 'FStar.Reflection.\*' StringPrinterTest.fst -skip-linking
