examples/tactics/StringPrinterTest.Aux.fst
@@ -1,0 +1,47 @@
+module StringPrinterTest.Aux
+include StringPrinter.RecC
+
+module Ca = FStar.Int.Cast
+module U32 = FStar.UInt32
+module T = FStar.Tactics
+module HST = FStar.HyperStack.ST
+module B = FStar.Buffer
+
+#reset-options "--use_two_phase_tc true --using_facts_from '* -FStar.Tactics -FStar.Reflection'"
+
+let rec example (x: U32.t) : Tot (m unit) (decreases (U32.v x)) =
+  _ <-- print_char (Ca.uint32_to_uint8 x) ;
+  if U32.lt x 256ul
+  then ret ()
+  else example (U32.div x 256ul)
+
+let example_do_while : (x: U32.t) -> Tot (y: m unit { y () == example x () } ) =
+  T.synth_by_tactic (fun () -> mk_do_while example )
+
+inline_for_extraction
+let example_sz (x: U32.t) : Tot (m_sz (example x)) =
+  coerce_sz
+    _
+    (example_do_while x)
+    (T.synth_by_tactic (fun () -> mk_sz 4 (example_do_while x)))
+    (example x)
+    ()
+
+inline_for_extraction
+let example_st (x: U32.t) : Tot (m_st (example x)) =
+  coerce_st
+    _
+    (example_do_while x)
+    (T.synth_by_tactic (fun () -> mk_st 4 (example_do_while x)))
+    (example x)
+    ()
+
+inline_for_extraction
+let example_test (x: U32.t) : HST.ST (option unit) (requires (fun _ -> True)) (ensures (fun h _ h' -> B.modifies_0 h h')) =
+  phi
+    (example x)
+    (example_sz x)
+    (example_st x)
+    ()
+
+let _ = T.assert_by_tactic True (fun () -> T.print "EOF")
